nondeterministic_dataflow/Spec.thy
@@ -1,0 +1,229 @@
+theory Spec
+
+imports
+  Operator
+  BNA_Operators
+begin
+
+corec spec_op where
+  "spec_op C = Choice (cimage (\<lambda> ios. case ios of
+    LNil \<Rightarrow> \<oslash> 
+  | LCons io ios' \<Rightarrow> 
+    (case io of
+      VInp p _ \<Rightarrow> Read p (\<lambda> y. spec_op (cimage ltl (cfilter (\<lambda> ios. lhd ios = VInp p y) C))) 
+    | VOut p x \<Rightarrow> Write (spec_op (cimage ltl (cfilter (\<lambda> ios. lhd ios = io) C))) p x)) C)"
+
+lemma step_spec_op_elim:
+  assumes  "step io (spec_op C) op"
+  obtains p x ios where "io = Out p x" "LCons (VOut p x) ios |\<in>| C" "op = spec_op (cimage ltl (cfilter (\<lambda> ios. lhd ios = VOut p x) C))"
+  | p x y ios where "io = Inp p y"  "LCons (VInp p x) ios |\<in>| C" "op = spec_op (cimage ltl (cfilter (\<lambda> ios. lhd ios = VInp p y) C))"
+  using assms apply -
+  apply atomize_elim
+  apply (subst (asm) spec_op.code)
+  apply (force split: llist.splits VIO.splits)
+  done
+
+lemma step_spec_op_intro1[intro]:
+  "C' = cimage ltl (cfilter (\<lambda> ios. lhd ios = VOut p x) C) \<Longrightarrow>
+   io = Out p x \<Longrightarrow>
+   (\<exists> ios. LCons (VOut p x) ios |\<in>| C) \<Longrightarrow>
+   step io (spec_op C) (spec_op C')"
+  apply hypsubst_thin
+  apply (elim exE)
+  apply (subst spec_op.code)
+  apply (rule SC)
+   apply (rule cimageI)
+   apply simp
+  apply force
+  done
+
+lemma step_spec_op_intro2[intro]:
+  "C' = cimage ltl (cfilter (\<lambda> ios. lhd ios = VInp p y) C) \<Longrightarrow>
+   io = Inp p y \<Longrightarrow>
+   (\<exists> ios x. LCons (VInp p x) ios |\<in>| C) \<Longrightarrow>
+   step io (spec_op C) (spec_op C')"
+  apply hypsubst_thin
+  apply (elim exE)
+  apply (subst spec_op.code)
+  apply (rule SC)
+   apply (rule cimageI)
+   apply simp
+  apply force
+  done
+
+lemma step_Tau_spec_op_False[simp]:
+  "\<not> (step Tau (spec_op C) op)"
+  apply (subst spec_op.code)
+  apply (auto split: llist.splits VIO.splits)
+  done
+
+corec repeat_op where
+  "repeat_op x = choice2
+   (Write (repeat_op x) (1 :: 1) x) (Silent (repeat_op x))"
+
+lemma step_repeat_op_elim:
+  assumes  "step io (repeat_op x) op"
+  obtains "io = Out 1 x" "op = repeat_op x"
+  | "io = Tau" "op = repeat_op x"
+  using assms apply -
+  apply atomize_elim
+  apply (subst (asm) repeat_op.code)
+  apply auto
+  done
+
+lemma step_repeat_intro[intro!]:
+  "io = Tau \<or> io = Out 1 x \<Longrightarrow>
+   step io (repeat_op x) (repeat_op x)"
+  apply (subst repeat_op.code)
+  apply auto
+  done
+
+lemma
+  "wtraced (repeat_op x) ios \<Longrightarrow>
+   ios = repeat (VOut 1 x)"
+  apply (coinduction arbitrary: ios)
+  subgoal for ios
+    apply (erule wtraced.cases)
+    subgoal
+      sorry
+    subgoal for vio op op' lxs
+      apply simp
+      apply hypsubst_thin
+      oops
+
+lemma
+  "wtraced (repeat_op x) (repeat (VOut 1 x))"
+  apply (coinduction)
+  apply simp
+  apply (rule disjI2)
+  apply (rule exI[of _ "VOut 1 x"])
+  apply (rule exI)
+  apply (rule exI[of _ "repeat (VOut 1 x)"])
+  apply simp
+  apply (intro conjI)
+    apply (meson iterates)
+   apply (rule step_wstep)
+   apply auto
+  done
+
+lemma repeat_op_spec_op:
+  "repeat_op x \<approx> spec_op {| repeat (VOut 1 x) |}"
+proof (coinduction rule: wbisim_coinduct)
+  case SIM1
+  then show ?case 
+    apply -
+    apply (elim step_repeat_op_elim; simp; hypsubst_thin?)
+    subgoal
+      apply (intro exI conjI wbcr_base step_wstep)
+        apply simp_all
+      apply (rule step_spec_op_intro1[where p=1])
+        apply simp_all
+       apply fastforce
+      apply (metis iterates)
+      done
+    subgoal
+      apply (intro exI conjI wbcr_base step_wstep)
+        apply simp_all
+      done
+    done
+next
+  case SIM2
+  then show ?case 
+    apply -
+    apply (elim step_spec_op_elim; simp; hypsubst_thin?)
+    subgoal
+      apply (intro exI conjI wbcr_base step_wstep)
+        apply simp_all
+       apply (metis io_of_vio.simps(2) lhd_iterates llist.sel(1) step_repeat_intro)
+      apply (smt (verit, ccfv_threshold) cimage_cempty cimage_cinsert cin_cfilter cset_eqI csingleton_iff lhd_LCons ltl_iterates)
+      done
+    subgoal
+      apply (intro exI conjI wbcr_base step_wstep)
+        apply simp_all
+       apply (metis VIO.distinct(1) lhd_LCons lhd_iterates)+
+      done
+    done
+qed
+
+lemma wstep_spec_opD:
+  "wstep (io_of_vio vio) (spec_op C) op' \<Longrightarrow>
+   step (io_of_vio vio) (spec_op C) op'"
+  apply (cases vio; simp)
+  subgoal
+    unfolding wstep_def
+    apply simp
+    apply (smt (verit) converse_rtranclpE relcomppE step_Tau_spec_op_False step_spec_op_elim)
+    done
+  subgoal
+    unfolding wstep_def
+    apply simp
+    apply (smt (verit) converse_rtranclpE relcomppE step_Tau_spec_op_False step_spec_op_elim)
+    done
+  done
+
+lemma wtraced_spec_op_soundness:
+  "ios |\<in>| C \<Longrightarrow>
+   wtraced (spec_op C) ios"
+  apply (coinduction arbitrary: ios C)
+  subgoal for ios
+    apply (cases ios)
+    subgoal
+      sorry
+    subgoal for io lxs
+      apply simp
+      apply (cases io; simp)
+      subgoal for p x
+        apply (intro conjI exI disjI1 step_wstep)
+          apply fastforce
+         apply (rule refl)
+        using cin_cimage_cfilter apply fastforce
+        done
+      subgoal
+        apply (intro conjI exI disjI1 step_wstep)
+          apply (rule step_spec_op_intro1)
+            apply simp_all
+         apply fast
+        apply force
+        done
+      done
+    done
+  done
+
+lemma wtraced_spec_op_completeness:
+  "wtraced (spec_op C) ios \<Longrightarrow>
+   ios |\<in>| C"
+  apply (erule wtraced.cases)
+  subgoal               
+    sorry
+  subgoal
+    apply hypsubst_thin
+
+  find_theorems "_ \<Longrightarrow> _ \<in> lset _" 
+
+lemma repeat_op_soundness:
+  "wtraced (repeat_op x) (repeat (VOut 1 x))"
+  by (metis cinsertCI repeat_op_spec_op wbisim_sym wbisim_wtraced wtraced_spec_op_soundness)
+
+lemma 
+  "wtraced (repeat_op x) ios \<Longrightarrow>
+   ios = repeat (VOut 1 x)"
+  oops
+
+
+
+end
+
+lemma
+  "sink_op = spec_op C"
+
+corec univ_source_op where
+  "univ_source_op = choice2
+   (Choice (cimage (\<lambda> n. Write univ_source_op (1 :: 1) (n :: _ :: countable)) cUNIV))
+   (Silent univ_source_op)"
+
+
+lemma
+  "univ_source_op \<approx> spec_op (cimage (lmap (VOut 1)) cUNIV)"
+
+
+end
